WIP

theories/examples/droe/deep_immutability_spec.v
@@ -14,7 +14,6 @@ Section DROE.
     `{MP: MachineParameters}
     {swlayout : switcherLayout}
   .
-  Context {C : CmptName}.
 
   Notation STS := (leibnizO (STS_states * STS_rels)).
   Notation STS_STD := (leibnizO (STS_std_states Addr region_type)).
@@ -28,6 +27,332 @@ Section DROE.
     (λne (W : WORLD) (B : leibnizO CmptName) (v : leibnizO Word)
      , (⌜ v = w ⌝ ∗ interp W B (readonly w))%I).
   Solve All Obligations with solve_proper.
+
+  Definition revoke_resources W C a :=
+    (∃ v φ p,
+      φ (W, C, v)
+      ∗ (monotonicity_guarantees_region C φ p v Temporary)
+      ∗ a ↦ₐ v
+      ∗ rcond (safeUC φ) C p interp
+      ∗ wcond (safeUC φ) C interp
+      ∗ rel C a p φ
+      ∗ ⌜ PermFlowsTo RWL p ⌝
+      ∗ ⌜ forall Wv, Persistent (φ Wv) ⌝)%I.
+
+  Lemma read_allowed_inv' (W : WORLD) (C : CmptName) (a b e: Addr) p g l :
+    readAllowed p →
+    Forall (fun a' : Addr => (b <= a' < e)%a ) l ->
+    ⊢ (interp W C (WCap p g b e a)) →
+    [∗ list] a' ∈ l,
+          (
+            ∃ (p' : Perm) (P:V),
+              ⌜ PermFlowsTo p p'⌝
+              ∗ ⌜persistent_cond P⌝
+              ∗ rel C a' p' (safeC P)
+              ∗ ▷ zcond P C
+              ∗ ▷ rcond P C p' interp
+              ∗ (if writeAllowed p' then (▷ wcond P C interp) else True)
+              ∗ monoReq W C a' p' P
+          ).
+  Proof.
+    induction l; iIntros (Hra Hin) "#Hinterp"; first done.
+    simpl.
+    apply Forall_cons in Hin. destruct Hin as [Hin_a0 Hin].
+    iDestruct (read_allowed_inv _ _ a0 with "Hinterp")
+      as (p' P) "(%Hperm_flow & %Hpers_P & Hrel_P & Hzcond_P & Hrcond_P & Hwcond_P & HmonoV)"
+    ; auto.
+    iFrame "%#".
+    iApply (IHl with "Hinterp"); eauto.
+  Qed.
+
+  Lemma writeLocalAllowed_valid_cap_implies (W : WORLD) (C : CmptName) p g b e a a':
+    isWL p = true ->
+    withinBounds b e a = true ->
+    interp W C (WCap p g b e a') -∗
+    ⌜std W !! a = Some Temporary⌝.
+  Proof.
+    intros Hp Hb. iIntros "Hinterp".
+    eapply withinBounds_le_addr in Hb.
+    rewrite fixpoint_interp1_eq interp1_eq; cbn.
+    replace (isO p) with false.
+    2: { eapply isWL_nonO in Hp ;done. }
+    destruct (has_sreg_access p) eqn:HnXSR; auto.
+    iDestruct "Hinterp" as "[Hinterp %Hloc]".
+    iDestruct (extract_from_region_inv with "Hinterp")
+             as (p' P' Hfl' Hpers') "(Hrel & Hzcond & Hrcond & Hwcond & HmonoR & %Hstate)";eauto.
+    by rewrite Hp in Hstate.
+  Qed.
+
+  Lemma writeLocalAllowed_valid_cap_implies' (W : WORLD) (C : CmptName) p g b e a l:
+    isWL p = true ->
+    Forall (fun a' : Addr => (b <= a' < e)%a ) l ->
+    ⊢ (interp W C (WCap p g b e a)) →
+    [∗ list] a' ∈ l, ⌜std W !! a' = Some Temporary⌝.
+  Proof.
+    induction l; iIntros (Hra Hin) "#Hinterp"; first done.
+    simpl.
+    apply Forall_cons in Hin; destruct Hin as [Hin_a0 Hin].
+    iDestruct (writeLocalAllowed_valid_cap_implies with "Hinterp") as "$"; auto.
+    { rewrite /withinBounds; solve_addr. }
+    iApply (IHl with "Hinterp"); eauto.
+  Qed.
+
+  Lemma read_allowed_inv_full_cap (W : WORLD) (C : CmptName) (a b e: Addr) p g :
+    readAllowed p →
+    ⊢ (interp W C (WCap p g b e a)) →
+    [∗ list] a' ∈ (finz.seq_between b e),
+          (
+            ∃ (p' : Perm) (P:V),
+              ⌜ PermFlowsTo p p'⌝
+              ∗ ⌜persistent_cond P⌝
+              ∗ rel C a' p' (safeC P)
+              ∗ ▷ zcond P C
+              ∗ ▷ rcond P C p' interp
+              ∗ (if writeAllowed p' then (▷ wcond P C interp) else True)
+              ∗ monoReq W C a' p' P
+          ).
+  Proof.
+    iIntros (Hra) "Hinterp".
+    iApply (read_allowed_inv' with "Hinterp"); eauto.
+    apply Forall_forall.
+    intros a' Ha'.
+    by apply elem_of_finz_seq_between.
+  Qed.
+
+  Lemma writeLocalAllowed_valid_cap_implies_full_cap (W : WORLD) (C : CmptName) p g b e a:
+    isWL p = true ->
+    ⊢ (interp W C (WCap p g b e a)) →
+    [∗ list] a' ∈ (finz.seq_between b e), ⌜std W !! a' = Some Temporary⌝.
+  Proof.
+    iIntros (Hwl) "Hinterp".
+    iApply (writeLocalAllowed_valid_cap_implies' with "Hinterp"); eauto.
+    apply Forall_forall.
+    intros a' Ha'.
+    by apply elem_of_finz_seq_between.
+  Qed.
+
+  Lemma monotone_revoke_list_sts_full_world_keep_interp W C (l : list Addr) (l' : list Addr) :
+    ⊢ ⌜NoDup l'⌝ → ⌜NoDup l⌝ → ⌜l' ⊆+ l⌝ →
+    ([∗ list] a' ∈ l',
+         ⌜(std W) !! a' = Some Temporary⌝ ∗
+          (
+            ∃ (p' : Perm) (P:V),
+              ⌜ PermFlowsTo RWL p'⌝
+              ∗ ⌜persistent_cond P⌝
+              ∗ rel C a' p' (safeC P)
+              ∗ ▷ zcond P C
+              ∗ ▷ rcond P C p' interp
+              ∗ (if writeAllowed p' then ▷ wcond P C interp else True)
+              ∗ monoReq W C a' p' P
+          ))
+    ∗ sts_full_world W C ∗ region W C
+    ==∗
+    (sts_full_world (revoke_list l W) C
+     ∗ region W C
+     ∗ ([∗ list] a' ∈ l', ▷ revoke_resources W C a')).
+  Proof.
+   rewrite region_eq /region_def /=.
+    iInduction (l) as [|x l] "IH" forall (l');
+    iIntros (Hdup' Hdup Hsub) "(#Hrel' & Hfull & Hr)".
+    - iFrame. apply submseteq_nil_r in Hsub as ->. repeat rewrite big_sepL_nil. done.
+    - destruct (decide (x ∈ l')).
+      + apply elem_of_list_split in e as [l1 [l2 Heq] ].
+        rewrite Heq in Hsub.
+        iRevert (Hsub Hdup Hdup'). rewrite Heq -Permutation_middle. iIntros (Hsub Hdup Hdup').
+        apply NoDup_cons in Hdup as [Hnin Hdup].
+        apply NoDup_cons in Hdup' as [Hnin' Hdup'].
+        assert (x ∈ l') as Ha.
+        { rewrite Heq. apply elem_of_app. right. apply elem_of_list_here. }
+        apply elem_of_Permutation in Ha as [l'' Hleq].
+        simpl. iDestruct "Hrel'" as "[ [%Htemp H] Hrel']".
+        iDestruct "H" as (p' P) "(%Hpermflow_p' & %Hpers_p' & #Hx & #Hzcond & #Hrcond & #Hwcond & #Hmono)".
+        iMod ("IH" with "[] [] [] [$Hrel' $Hfull $Hr]") as "(Hfull & Hr & Hl)"; auto.
+        { iPureIntro. apply submseteq_cons_l in Hsub as [k' [Hperm Hsub] ].
+          apply Permutation.Permutation_cons_inv in Hperm. etrans;eauto. rewrite Hperm. done. }
+        rewrite /revoke_list /= /=.
+        rewrite Htemp.
+        rewrite rel_eq /rel_def.
+        iDestruct "Hr" as (M Mρ) "(HM & % & #Hdom & Hpreds)".
+        iDestruct "Hdom" as %Hdom.
+        iDestruct "Hx" as (γpred) "#(Hγpred & Hφ)".
+        iDestruct ( (reg_in C M) with "[$HM $Hγpred]") as %HMeq; auto.
+        rewrite /region_map_def.
+        rewrite HMeq big_sepM_insert; [|by rewrite lookup_delete].
+        iDestruct "Hpreds" as "[Ha Hpreds]".
+        iDestruct "Ha" as (ρ Ha) "[Hstate Ha]".
+        iDestruct (sts_full_state_std with "Hfull Hstate") as %Hlookup.
+        simpl in Hlookup.
+        simpl in Hlookup. subst. rewrite revoke_list_not_elem_of_lookup in Hlookup; auto.
+        rewrite Htemp in Hlookup. inversion Hlookup. subst ρ.
+        iMod (sts_update_std _ _ _ _ (Revoked) with "Hfull Hstate") as "[Hfull Hstate]".
+        iDestruct (region_map_delete with "Hpreds") as "Hpreds".
+        iDestruct (region_map_insert _ _ _ _ _ Revoked with "Hpreds") as "Hpreds";auto.
+        iDestruct (big_sepM_insert _ _ x (γpred, p') with "[$Hpreds Hstate]") as "Hpreds"
+        ; [apply lookup_delete|..]
+        ; iClear "IH"
+        ; iFrame "∗ #".
+        iSplitR;[iPureIntro; apply lookup_insert|].
+        iExists _ ;iSplit;auto.
+        rewrite -HMeq.
+        iModIntro. iSplitR.
+        ++ iSplit; auto.
+           iPureIntro. rewrite dom_insert_L.
+           assert (x ∈ dom M) as Hin.
+           { rewrite -Hdom. apply elem_of_dom. eauto. }
+           revert Hin Hdom. clear; intros Hin Hdom. rewrite Hdom. set_solver.
+        ++ iFrame "∗#%".
+           iDestruct "Ha" as (γpred0 p0 φ0 Heq0 Hpers0) "(#Hsaved & Ha)".
+           iDestruct "Ha" as (v Hne0) "(Hx & #HmonoV & #Hφ0)"; simplify_eq.
+           iFrame "∗#%".
+           destruct W as [ Wstd_sta Wloc].
+           iDestruct (saved_pred_agree _ _ _ _ _ (Wstd_sta, Wloc, C, v) with "Hφ Hsaved") as "#Hφeq". iFrame.
+           iDestruct (internal_eq_iff with "Hφeq") as "Hφeq'".
+           iDestruct ("Hφeq'" with "Hφ0") as "HP"; iFrame "HP".
+           rewrite rel_eq /rel_def; iFrame "Hγpred Hφ".
+           rewrite /monotonicity_guarantees_region.
+           iSplit.
+           {
+             destruct (isWL p0).
+             +++ iApply future_pub_mono_eq_pred; auto.
+             +++ destruct (isDL p0).
+                 ++++ iApply future_borrow_mono_eq_pred; auto.
+                 ++++ iApply future_priv_mono_eq_pred; auto.
+           }
+           { destruct p0.
+             destruct rx,w; cbn in *; try done.
+           }
+      + apply NoDup_cons in Hdup as [Hnin Hdup].
+        apply submseteq_cons_r in Hsub as [Hsub | [l'' [Hcontr _] ] ].
+        2: { exfalso. apply n. rewrite Hcontr. apply elem_of_list_here. }
+        iMod ("IH" with "[] [] [] [$Hrel' $Hfull $Hr]") as "(Hfull & Hr & Hl)"; auto.
+        iDestruct "Hr" as (M Mρ) "(HM & #Hdom & #Hdom' & Hr)".
+        iDestruct "Hdom" as %Hdom. iDestruct "Hdom'" as %Hdom'. iClear "IH".
+        rewrite /revoke_list /=. destruct W as [ Wstd_sta Wloc].
+        destruct (Wstd_sta !! x) eqn:Hsome.
+        2: { iFrame. iModIntro. rewrite Hsome. iFrame. auto. }
+        rewrite Hsome.
+        destruct (decide (r = Temporary)).
+        2: { destruct r; try contradiction; iFrame; iModIntro; iFrame; auto. }
+        assert (is_Some (M !! x)) as [γp Hsomea].
+        { apply elem_of_dom. rewrite -Hdom. rewrite elem_of_dom. eauto. }
+        iDestruct (big_sepM_delete _ _ x with "Hr") as "[Hx Hr]"; eauto.
+        iDestruct "Hx" as (ρ Ha) "[Hstate Hρ]".
+        iDestruct (sts_full_state_std with "Hfull Hstate") as %Hlookup.
+        iMod (sts_update_std _ _ _ _ (Revoked) with "Hfull Hstate") as "[Hfull Hstate]".
+        iDestruct (region_map_delete with "Hr") as "Hpreds".
+        simplify_map_eq.
+        simpl in *. rewrite revoke_list_not_elem_of_lookup in Hlookup;auto.
+        rewrite Hlookup in Hsome. inversion Hsome. subst.
+        iDestruct (region_map_insert _ _ _ _ _ Revoked with "Hpreds") as "Hpreds";auto.
+        iDestruct (big_sepM_delete _ _ x with "[Hstate $Hpreds Hρ]") as "Hr"; eauto.
+        iExists Revoked; iSplitR; first (by iPureIntro ; simplify_map_eq).
+        iFrame.
+        iDestruct "Hρ" as (? ? ? ? ?) "[? _]". iExists _,_,_. repeat iSplit;eauto.
+        iModIntro. iFrame.
+        iSplit; auto.
+        iPureIntro. rewrite dom_insert_L.
+        assert (x ∈ dom M) as Hin.
+        { rewrite -Hdom'. apply elem_of_dom. eauto. }
+        revert Hin Hdom'. clear; intros Hin Hdom. rewrite Hdom. set_solver.
+  Qed.
+
+  Lemma monotone_revoke_sts_full_world_keep_interp W C (l : list Addr) :
+    ⌜NoDup l⌝ -∗
+    ([∗ list] a' ∈ l,
+         ⌜(std W) !! a' = Some Temporary⌝ ∗
+          (
+            ∃ (p' : Perm) (P:V),
+              ⌜ PermFlowsTo RWL p'⌝
+              ∗ ⌜persistent_cond P⌝
+              ∗ rel C a' p' (safeC P)
+              ∗ ▷ zcond P C
+              ∗ ▷ rcond P C p' interp
+              ∗  (if writeAllowed p' then ▷ wcond P C interp else True)
+              ∗ monoReq W C a' p' P
+          ))
+    ∗ sts_full_world W C ∗ region W C
+    ==∗
+    (sts_full_world (revoke W) C
+     ∗ region W C
+     ∗ ([∗ list] a' ∈ l, ▷ revoke_resources W C a')).
+  Proof.
+    iIntros (Hdup) "(Hl & Hfull & Hr)".
+    rewrite revoke_list_dom.
+    iAssert (⌜l ⊆+ (map_to_list (std W)).*1⌝)%I as %Hsub.
+    { iClear "Hfull Hr". iInduction l as [| x l] "IH".
+      - iPureIntro. apply submseteq_nil_l.
+      - iDestruct "Hl" as "[ [Hin Hrel] Hl]".
+        iDestruct "Hin" as %Hin. apply NoDup_cons in Hdup as [Hnin Hdup].
+        iDestruct ("IH" with "[] Hl") as %Hsub; auto.
+        iPureIntro.
+        assert (x ∈ (map_to_list (std W)).*1) as Helem.
+        { apply map_to_list_fst. exists Temporary. by apply elem_of_map_to_list. }
+        apply elem_of_Permutation in Helem as [l' Hl']. rewrite Hl'.
+        apply submseteq_skip. revert Hsub. rewrite Hl'; intros Hsub.
+        apply submseteq_cons_r in Hsub as [Hsub | [l'' [Heq _] ] ]; auto.
+        assert (x ∈ l) as Hcontr.
+        { rewrite Heq. apply elem_of_list_here. }
+        subst. contradiction.
+    }
+    iMod (monotone_revoke_list_sts_full_world_keep_interp _ _ (map_to_list (std W)).*1 l
+            with "[] [] [] [Hl $Hfull $Hr]") as "(Hfull & Hr & Hi)"; auto.
+    { iPureIntro. apply (NoDup_fst_map_to_list (M:=gmap Addr) (A:=region_type)). }
+    by iFrame.
+  Qed.
+
+  (* revoke stack, with unknown p and φ *)
+  Lemma monotone_revoke_stack W C b e a :
+    let la := finz.seq_between b e in
+
+    interp W C (WCap RWL Local b e a)
+    ∗ sts_full_world W C
+    ∗ region W C
+    ==∗
+    sts_full_world (revoke W) C
+    ∗ region (revoke W) C
+    ∗ ([∗ list] a ∈ la, ▷ revoke_resources W C a ∗ ⌜(std (revoke W)) !! a = Some Revoked⌝).
+  Proof.
+    iIntros (la) "(#Hinterp & HW & Hr)".
+    iAssert (
+       ([∗ list] a' ∈ la,
+         ⌜(std W) !! a' = Some Temporary⌝ ∗
+          (
+            ∃ (p' : Perm) (P:V),
+              ⌜ PermFlowsTo RWL p'⌝
+              ∗ ⌜persistent_cond P⌝
+              ∗ rel C a' p' (safeC P)
+              ∗ ▷ zcond P C
+              ∗ ▷ rcond P C p' interp
+              ∗ (if writeAllowed p' then ▷ wcond P C interp else True)
+              ∗ monoReq W C a' p' P
+          ))%I
+      ) with "[Hinterp]" as "Hl".
+    {
+      iDestruct (writeLocalAllowed_valid_cap_implies_full_cap with "Hinterp") as "Htmp"; first done.
+      iDestruct (read_allowed_inv_full_cap with "Hinterp") as "H"; first done.
+      iApply big_sepL_sep; iFrame "#".
+    }
+    iAssert (⌜Forall (λ a, std W !! a = Some Temporary) la⌝)%I as %Htemps.
+    { iDestruct (big_sepL_sep with "Hl") as "[Htemps Hrel]".
+      iDestruct (big_sepL_forall with "Htemps") as %Htemps.
+      iPureIntro. apply Forall_lookup. done. }
+    iMod (monotone_revoke_sts_full_world_keep_interp with "[] [$HW $Hr $Hl]") as "(HW & Hr & Hl')"; eauto.
+    { iPureIntro ; subst la ; apply finz_seq_between_NoDup. }
+    rewrite region_eq /region_def.
+    iDestruct "Hr" as (M Mρ) "(HM & %Hdom & % & Hpreds)".
+    iDestruct (monotone_revoke_region_def with "[] [$HW] [$Hpreds]") as "[Hpreds HW]"; auto.
+    iModIntro. iFrame. iSplitR.
+    - iPureIntro.
+      rewrite /revoke in Hdom |- *.
+      repeat (split;auto).
+      by rewrite -revoke_dom_eq.
+    - iApply big_sepL_sep. iFrame. iApply big_sepL_forall. iPureIntro.
+      revert Htemps. rewrite (Forall_lookup _ la). intros Hl i a' Ha; auto.
+      specialize (Hl i a' Ha).
+      rewrite /revoke in Hdom, Hl |- *.
+      by apply revoke_lookup_Monotemp.
+  Qed.
+
 
   Lemma droe_spec
 
@@ -438,32 +763,6 @@ Section DROE.
 
     Set Nested Proofs Allowed.
     (* TODO move *)
-    Lemma is_switcher_entry_point_call :
-     is_switcher_entry_point (WSentry XSRW_ Local b_switcher e_switcher a_switcher_call) = true.
-    Proof.
-      rewrite /is_switcher_entry_point.
-      rewrite bool_decide_eq_true_2; first done.
-      by left.
-    Qed.
-    Lemma is_switcher_entry_point_return :
-     is_switcher_entry_point (WSentry XSRW_ Local b_switcher e_switcher a_switcher_return) = true.
-    Proof.
-      rewrite /is_switcher_entry_point.
-      rewrite bool_decide_eq_true_2; first done.
-      by right.
-    Qed.
-    Lemma switcher_call_interp W B :
-     ⊢ interp W B (WSentry XSRW_ Local b_switcher e_switcher a_switcher_call).
-    Proof.
-      iEval (rewrite fixpoint_interp1_eq /=).
-      by rewrite is_switcher_entry_point_call.
-    Qed.
-    Lemma switcher_return_interp W B :
-     ⊢ interp W B (WSentry XSRW_ Local b_switcher e_switcher a_switcher_return).
-    Proof.
-      iEval (rewrite fixpoint_interp1_eq /=).
-      by rewrite is_switcher_entry_point_return.
-    Qed.
 
     iAssert ([∗ map] rarg↦warg ∈ rmap_arg, rarg ↦ᵣ warg ∗ interp W2 C warg )%I
       with "[Hca0 Hca1 Hca2 Hca3 Hca4 Hca5 Hct0]" as "Hrmap_arg".
